Isabelle/Grammar.thy
@@ -536,7 +536,7 @@ lemma nov_distr_cons:
   "norm_of_variables gr (x # y) = norm_of_variables gr [x] + norm_of_variables gr y"
 by (rule nov_distr[of _ "[x]", simplified])
 
-lemma nov_singleton: "norm_of_variables gr [v] = fst (lookup (norms_of_grammar gr) v)"
+lemma nov_singleton: "norm_of_variables gr [v] = fst (lookup (norms_of_grammar2 gr) v)"
 by (simp add: norm_of_variables_def ns_singleton)
 
 lemma nov_mnor:
@@ -593,7 +593,7 @@ qed*)
 sorry
 
 
-lemma nov_nog':
+(*lemma nov_nog':
   assumes "gram_sd gr"
       and "(v, n, t, vs) \<in> set (norms_of_grammar gr)"
       and "(v, rules) \<in> set gr"
@@ -636,14 +636,14 @@ proof -
 
   def n \<equiv> "fst (lookup (norms_of_grammar gr) v)"
   then show ?thesis using G nov_nog'[of gr v n t] existence_from_lookup[OF A V] assms n_def by auto
-qed
+qed*)
 
 lemma nov_greater_zero:
-  assumes "gram_nsd gr"
+  assumes "gram_nsd2 gr"
       and "set v \<subseteq> keys gr"
       and "v \<noteq> []"
     shows "0 < norm_of_variables gr v" using assms unfolding norm_of_variables_def
-by (induct v) (auto, subst ns_distr_cons, simp add: ns_singleton nog_greater_zero_lookup)
+by (induct v) (auto, subst ns_distr_cons, simp add: ns_singleton nog2_greater_zero_lookup)
 
 lemma nov_empty: "norm_of_variables gr [] = 0"
 by (simp add: norm_of_variables_def ns_empty)
@@ -656,38 +656,38 @@ by (simp add: norm_of_variables_def ns_empty)
 termination minimal_word_of_variables
   apply (relation "measure (\<lambda>(gr, vs). norm_of_variables gr vs)", auto)
   apply (subst nov_distr_cons)
-  apply (auto simp add: add_commute add_strict_increasing2 nov_nog)
+  apply (auto simp add: add_commute add_strict_increasing2 nov_nog2)
   apply (subst nov_distr_cons)
 by (auto simp add: nov_greater_zero)
 
 lemmas mwov_induct = minimal_word_of_variables.induct[case_names Nil_vars Cons_vars]
 
 lemma mwov_dist:
-  assumes "gram_nsd gr"
+  assumes "gram_nsd2 gr"
       and "set v1 \<subseteq> keys gr"
       and "set v2 \<subseteq> keys gr"
     shows "minimal_word_of_variables gr (v1 @ v2) =
            minimal_word_of_variables gr v1 @ minimal_word_of_variables gr v2" using assms
 proof (induct v1 arbitrary: v2)
   case (Cons a v1)
-  then show ?case by (case_tac "snd (lookup (norms_of_grammar gr) a)") auto
+  then show ?case by (case_tac "snd (lookup (norms_of_grammar2 gr) a)") auto
 qed auto
 
 lemma mwov_len_calcs_nog:
-  assumes "gram_nsd gr"
+  assumes "gram_nsd2 gr"
       and "v \<in> keys gr"
-      and "(n, nt, nrt) = lookup (norms_of_grammar gr) v"
+      and "(n, nt, nrt) = lookup (norms_of_grammar2 gr) v"
     shows "Suc (length (minimal_word_of_variables gr nrt)) = n" using assms
 sorry
 
 theorem mwov_len_calcs_nov:
-  assumes G: "gram_nsd gr"
+  assumes G: "gram_nsd2 gr"
       and V: "set v \<subseteq> fst ` set gr"
     shows "length (minimal_word_of_variables gr v) = norm_of_variables gr v" using assms
 proof (induct gr v rule: mwov_induct)
   case (Cons_vars gr vh vt)
 
-  def nogh \<equiv> "lookup (norms_of_grammar gr) vh"
+  def nogh \<equiv> "lookup (norms_of_grammar2 gr) vh"
   def nh   \<equiv> "fst nogh"
   def trh  \<equiv> "snd nogh"
   def th   \<equiv> "fst trh"
@@ -720,27 +720,27 @@ proof (induct gr v rule: mwov_induct)
 qed (simp add: nov_empty)
 
 lemma mwov_empty:
-  assumes "gram_nsd gr"
+  assumes "gram_nsd2 gr"
       and "set v \<subseteq> fst ` set gr"
       and "minimal_word_of_variables gr v = []"
     shows "v = []" using assms
 proof (induct v)
   case (Cons a v)
-  then show ?case by (case_tac "snd (lookup (norms_of_grammar gr) a)") auto
+  then show ?case by (case_tac "snd (lookup (norms_of_grammar2 gr) a)") auto
 qed auto
 
 lemma mwov_length_singleton:
-  assumes "gram_nsd gr"
+  assumes "gram_nsd2 gr"
       and "(vh, rules) \<in> set gr"
       and "(th, rth) \<in> set rules"
     shows "length (minimal_word_of_variables gr [vh]) \<le>
        1 + length (minimal_word_of_variables gr rth)" using assms
-  apply (case_tac "snd (lookup (norms_of_grammar gr) vh)")
+  apply (case_tac "snd (lookup (norms_of_grammar2 gr) vh)")
   apply auto
 sorry
 
 lemma mwov_length:
-  assumes G: "gram_nsd gr"
+  assumes G: "gram_nsd2 gr"
       and T: "set vt \<subseteq> keys gr"
       and V: "(vh, rules) \<in> set gr"
       and R: "(th, rth) \<in> set rules"
@@ -756,37 +756,37 @@ proof -
     using mwov_dist G VH T .
   have D2: "minimal_word_of_variables gr (rth @ vt) =
             minimal_word_of_variables gr rth @ minimal_word_of_variables gr vt"
-    using mwov_dist G gram_rule_vars_in_keys[OF gram_nsd_sd[OF G] V R] T .
+    using mwov_dist G gram_rule_vars_in_keys[OF gram_nsd2_sd[OF G] V R] T .
 
   show ?thesis using L D1 D2 by auto
 qed
 
 lemma mwov_hd_from_nog:
-  assumes "gram_nsd gr"
+  assumes "gram_nsd2 gr"
       and "(vh, rules) \<in> set gr"
       and "set vt \<subseteq> keys gr"
       and "th # tt = minimal_word_of_variables gr (vh # vt)"
-    shows "th = fst (snd (lookup (norms_of_grammar gr) vh))" using assms
-by (case_tac "snd (lookup (norms_of_grammar gr) vh)") auto
+    shows "th = fst (snd (lookup (norms_of_grammar2 gr) vh))" using assms
+by (case_tac "snd (lookup (norms_of_grammar2 gr) vh)") auto
 
 lemma mwov_prefix:
-  assumes G: "gram_nsd gr"
+  assumes G: "gram_nsd2 gr"
       and V: "(vh, rules) \<in> set gr"
       and S: "set vt \<subseteq> keys gr"
       and M: "th # tt = minimal_word_of_variables gr (vh # vt)"
     shows "tt = minimal_word_of_variables gr ((lookup rules th) @ vt)"
 proof -
   def rth  \<equiv> "lookup rules th"
-  def nvh  \<equiv> "snd (lookup (norms_of_grammar gr) vh)"
+  def nvh  \<equiv> "snd (lookup (norms_of_grammar2 gr) vh)"
   def nth  \<equiv> "fst nvh"
   def nrth \<equiv> "snd nvh"
 
   have "th = nth" using assms by (auto simp add: nth_def nvh_def mwov_hd_from_nog)
-  then have SL: "snd (lookup (norms_of_grammar gr) vh) = (th, nrth)"
+  then have SL: "snd (lookup (norms_of_grammar2 gr) vh) = (th, nrth)"
     using nvh_def nrth_def nth_def by auto
 
-  have GS: "gram_sd gr" using G by (rule gram_nsd_sd)
-  have TN: "(th, nrth) \<in> set rules" using nog_in_rules[OF G V] SL by simp
+  have GS: "gram_sd gr" using G by (rule gram_nsd2_sd)
+  have TN: "(th, nrth) \<in> set rules" using nog2_in_rules[OF G V] SL by simp
   have LO: "lookup rules th = nrth"
     using lookup_from_existence gram_rules_alist[OF GS V] TN .
 
@@ -855,7 +855,7 @@ proof -
 qed
 
 lemma wiv_mwov:
-  assumes G: "gram_nsd gr"
+  assumes G: "gram_nsd2 gr"
       and V: "set v \<subseteq> keys gr"
     shows "word_in_variables gr (minimal_word_of_variables gr v) v" using assms
 proof (induct gr "(minimal_word_of_variables gr v)" v rule: eat_word_induct)
@@ -863,18 +863,18 @@ proof (induct gr "(minimal_word_of_variables gr v)" v rule: eat_word_induct)
 
   def rules \<equiv> "lookup gr vh"
   def   rth \<equiv> "lookup rules th"
-  def  nrth \<equiv> "snd (snd (lookup (norms_of_grammar gr) vh))"
+  def  nrth \<equiv> "snd (snd (lookup (norms_of_grammar2 gr) vh))"
 
-  have GS: "gram_sd gr" using normal by (simp add: gram_nsd_sd)
+  have GS: "gram_sd gr" using normal by (simp add: gram_nsd2_sd)
   have VT: "set vt \<subseteq> keys gr" using normal(4) by simp
   have VR: "(vh, rules) \<in> set gr" using gram_alist[OF GS] normal rules_def
     by (simp add: existence_from_lookup)
   have RA: "is_alist rules" using gram_rules_alist GS VR .
 
-  have "th = fst (snd (lookup (norms_of_grammar gr) vh))"
+  have "th = fst (snd (lookup (norms_of_grammar2 gr) vh))"
     using mwov_hd_from_nog normal(3) VR VT normal(2) .
-  then have TN: "(th, nrth) = snd (lookup (norms_of_grammar gr) vh)" using nrth_def by simp
-  have TH: "th \<in> keys rules" using nog_in_rules [OF normal(3) VR] TN[symmetric] by simp
+  then have TN: "(th, nrth) = snd (lookup (norms_of_grammar2 gr) vh)" using nrth_def by simp
+  have TH: "th \<in> keys rules" using nog2_in_rules [OF normal(3) VR] TN[symmetric] by simp
 
   have TT: "tt = minimal_word_of_variables gr (rth @ vt)" unfolding rth_def
     using mwov_prefix normal(3) VR VT normal(2) .
@@ -889,7 +889,7 @@ lemma wiv_word_head: "word_in_variables gr (th # tt) (vh # vt) \<Longrightarrow>
 by (case_tac "th \<in> keys (lookup gr vh)") (auto simp add: Let_def word_in_variables_def)
 
 lemma mwov_minimal_wiv:
-  assumes "gram_nsd gr"
+  assumes "gram_nsd2 gr"
       and "set v \<subseteq> keys gr"
       and "word_in_variables gr w v"
     shows "length (minimal_word_of_variables gr v) \<le> length w" using assms
@@ -899,7 +899,7 @@ proof (induct gr w v rule: eat_word_induct)
   def rules \<equiv> "lookup gr vh"
   def   rth \<equiv> "lookup rules th"
 
-  have GS: "gram_sd gr" using normal by (simp add: gram_nsd_sd)
+  have GS: "gram_sd gr" using normal by (simp add: gram_nsd2_sd)
   have VR: "(vh, rules) \<in> set gr" using GS normal rules_def
     by (simp add: existence_from_lookup gram_alist)
   have RA: "is_alist rules" using gram_rules_alist GS VR .
@@ -923,13 +923,13 @@ qed (auto simp add: word_in_variables_def)
  *****************************************************************************)
 
 lemma mwov_in_wov:
-  assumes "gram_nsd gr"
+  assumes "gram_nsd2 gr"
       and "set v \<subseteq> keys gr"
     shows "minimal_word_of_variables gr v \<in> words_of_variables gr v" using assms
 by (simp add: words_of_variables_def wiv_mwov)
 
 lemma mwov_min_wov:
-  assumes "gram_nsd gr"
+  assumes "gram_nsd2 gr"
       and "set v \<subseteq> keys gr"
     shows "w \<in> words_of_variables gr v \<Longrightarrow> length (minimal_word_of_variables gr v) \<le> length w"
 using assms by (auto simp add: words_of_variables_def mwov_minimal_wiv)
@@ -940,13 +940,13 @@ using assms by (auto simp add: words_of_variables_def mwov_minimal_wiv)
  *****************************************************************************)
 
 theorem mwov_len_calcs_norm:
-  assumes "gram_nsd gr"
+  assumes "gram_nsd2 gr"
       and "set v \<subseteq> keys gr"
     shows "norm gr v = length (minimal_word_of_variables gr v)" using assms unfolding norm_def
 by (auto intro: Least_equality simp add: mwov_min_wov mwov_in_wov)
 
 theorem nov_calculates_norm:
-  assumes "gram_nsd gr"
+  assumes "gram_nsd2 gr"
       and "set v \<subseteq> keys gr"
     shows "norm_of_variables gr v = norm gr v" using assms
 by (auto simp add: mwov_len_calcs_norm mwov_len_calcs_nov)
