Isabelle/Tests.thy
@@ -17,20 +17,20 @@ definition test_gr3 :: "(char, nat) grammar" where
   "test_gr3 =
    [(0, [(CHR ''a'', [0])])]"
 
-value "gram_nsd test_gr"
+value "gram_nsd2 test_gr"
 value "gram_max_vars test_gr = 1"
 value "norm_of_variables test_gr [0] = 1"
 value "norm_of_variables test_gr [1] = 2"
 value "word_in_variables test_gr ''a'' [0]"
 value "minimal_word_of_variables test_gr [1] = ''ba''"
 
-value "gram_nsd test_gr2"
+value "gram_nsd2 test_gr2"
 value "norm_of_variables test_gr2 [0] = 1"
 value "norm_of_variables test_gr2 [1] = 2"
 value "norm_of_variables test_gr2 [2] = 2"
 value "norm_of_variables test_gr2 [3] = 1"
 
 value "gram_sd test_gr3"
-value "gram_nsd test_gr3 = False"
+value "gram_nsd2 test_gr3 = False"
 
 end
